merge modification Benj + Laurent

num/GenDivn1.v
@@ -1,9 +1,11 @@
 Set Implicit Arguments.
 
 Require Import ZArith.
-Require Import Basic_type.
 Require Import ZDivModAux.
 Require Import ZPowerAux.
+Require Import Basic_type.
+Require Import GenBase.
+
 Open Local Scope Z_scope.
 
 Section GENDIVN1.
@@ -17,21 +19,22 @@ Section GENDIVN1.
  Variable w_div21       : w -> w -> w -> w * w.
  
  (* ** For proofs ** *)
- 
- Let wB := base w_digits. 
  Variable w_to_Z        : w -> Z.
+ 
+ Notation wB := (base w_digits). 
+
  Notation "[| x |]" := (w_to_Z x)  (at level 0, x at level 99).
  Notation "[! n | x !]" := (gen_to_Z w_digits w_to_Z n x) 
                                       (at level 0, x at level 99).
- Notation "[|| x ||]" := (zn2z_to_Z wB w_to_Z x)  (at level 0, x at level 99).
+ Notation "[[ x ]]" := (zn2z_to_Z wB w_to_Z x)  (at level 0, x at level 99).
  
  Variable spec_to_Z   : forall x, 0 <= [| x |] < wB.
  Variable spec_0   : [|w_0|] = 0.
- Variable spec_WW  : forall h l, [||w_WW h l||] = [|h|] * wB + [|l|].
+ Variable spec_WW  : forall h l, [[w_WW h l]] = [|h|] * wB + [|l|].
  Variable spec_head0  : forall x,  0 < [|x|] ->
 	 wB/ 2 <= 2 ^ (Z_of_N (w_head0 x)) * [|x|] < wB.
  Variable spec_add_mul_div : forall x y p,
-       Zpos p < Zpos w_digits ->
+        Zpos p < Zpos w_digits ->
        [| w_add_mul_div p x y |] =
          ([|x|] * (Zpower 2 (Zpos p)) +
           [|y|] / (Zpower 2 ((Zpos w_digits) - (Zpos p)))) mod wB.
@@ -41,70 +44,27 @@ Section GENDIVN1.
      let (q,r) := w_div21 a1 a2 b in
      [|a1|] *wB+ [|a2|] = [|q|] * [|b|] + [|r|] /\
      0 <= [|r|] < [|b|].
-
- Definition genWW (n:nat) := 
-  match n return word w n -> word w n -> word w (S n) with 
-  | O => w_WW 
-  | S n =>
-    fun (h l : zn2z (word w n)) =>
-     match h, l with
-     | W0, W0 => W0
-     | _, _ => WW h l
-     end
-  end.
-
- Lemma spec_genWW : forall n (h l : word w n),
-   [!S n|genWW n h l!] = [!n|h!] * gen_wB w_digits n + [!n|l!].
- Proof.
-  induction n;simpl;intros;trivial.
-  destruct h;auto.
-  destruct l;auto.
- Qed.
-
-
- Definition gen0 (n:nat) : word w n :=
-  match n return (word w n) with
-  | O => w_0
-  | S n => W0
-  end.
  
- Lemma spec_gen0 : forall n, [!n|gen0 n!] = 0.
- Proof.
-  destruct n;simpl;auto.
- Qed.
-
- Definition split (n:nat) (x:zn2z (word w n)) :=
-  match x with 
-  | W0 => let w0 := gen0 n in (w0,w0)
-  | WW h l => (h,l)
-  end.
-
- Lemma spec_split : forall n (x:zn2z (word w n)),
-   let (h,l) := split n x in
-   [!S n|x!] = [!n|h!] * gen_wB w_digits n + [!n|l!].
- Proof.
-  destruct n;simpl;intros.
-  destruct x;simpl;auto.
-  rewrite spec_0;trivial.
-  destruct x;simpl;auto.
- Qed.
-
  Section DIVAUX.
   Variable b2p : w.
   Variable b2p_le : wB/2 <= [|b2p|].
 
-  Fixpoint gen_divn1_0 (n:nat) (r:w) {struct n} : 
-	          word w n -> word w n * w :=
-   match n return word w n -> word w n * w with
-   | O => fun x => w_div21 r x b2p 
-   | S n =>
-     fun (h:zn2z (word w n)) =>
-      let (hh,hl) := split n h in
-      let (qh,rh) := gen_divn1_0 n r hh in
-      let (ql,rl) := gen_divn1_0 n rh hl in
-      (genWW n qh ql, rl)
+  Definition gen_divn1_0_aux n (divn1: w -> word w n -> word w n * w) r h :=
+   let (hh,hl) := gen_split w_0 n h in
+   let (qh,rh) := divn1 r hh in
+   let (ql,rl) := divn1 rh hl in
+   (gen_WW w_WW n qh ql, rl).
+
+  Fixpoint gen_divn1_0 (n:nat) : w -> word w n -> word w n * w :=
+   match n return w -> word w n -> word w n * w with
+   | O => fun r x => w_div21 r x b2p 
+   | S n => gen_divn1_0_aux n (gen_divn1_0 n) 
    end.
-  
+ 
+  Lemma spec_split : forall (n : nat) (x : zn2z (word w n)),
+       let (h, l) := gen_split w_0 n x in
+       [!S n | x!] = [!n | h!] * gen_wB w_digits n + [!n | l!].
+  Proof (spec_gen_split w_0 w_digits w_to_Z spec_0).
 
   Lemma spec_gen_divn1_0 : forall n r a,
     [|r|] < [|b2p|] ->
@@ -114,84 +74,71 @@ Section GENDIVN1.
   Proof.
    induction n;intros.
    exact (spec_div21 a b2p_le H).
-   unfold gen_divn1_0;fold gen_divn1_0.
-   assert (H1 := spec_split n a);destruct (split n a) as (hh,hl).
+   unfold gen_divn1_0, gen_divn1_0_aux;fold gen_divn1_0.
+   assert (H1 := spec_split n a);destruct (gen_split w_0 n a) as (hh,hl).
    rewrite H1.
    assert (H2 := IHn r hh H);destruct (gen_divn1_0 n r hh) as (qh,rh).
    destruct H2.
    assert ([|rh|] < [|b2p|]). omega.
    assert (H4 := IHn rh hl H3);destruct (gen_divn1_0 n rh hl) as (ql,rl).
    destruct H4;split;trivial.
-   rewrite spec_genWW.
+   rewrite spec_gen_WW;trivial.
    rewrite <- gen_wB_wwB.
-   replace 
-   ([|r|] * (gen_wB w_digits n * gen_wB w_digits n) + 
-       ([!n|hh!] * gen_wB w_digits n + [!n|hl!]))
-   with
-   ((([|r|] * gen_wB w_digits n) + [!n|hh!]) * gen_wB w_digits n + [!n|hl!]).
-   2:ring.
-   rewrite H0.
-   replace (([!n|qh!] * [|b2p|] + [|rh|]) * gen_wB w_digits n + [!n|hl!]) 
-   with
-   (([!n|qh!] * [|b2p|]*gen_wB w_digits n) + 
-       ([|rh|]*gen_wB w_digits n + [!n|hl!])).
-   2:ring.
+   rewrite Zmult_assoc;rewrite Zplus_assoc;rewrite <- Zmult_plus_distr_l.
+   rewrite H0;rewrite Zmult_plus_distr_l;rewrite <- Zplus_assoc.
    rewrite H4;ring.
   Qed.
 
-  Fixpoint gen_modn1_0 (n:nat) (r:w) {struct n} : 
-	          word w n -> w :=
-   match n return word w n -> w with
-   | O => fun x => snd (w_div21 r x b2p)
-   | S n =>
-     fun (h:zn2z (word w n)) =>
-      let (hh,hl) := split n h in
-      gen_modn1_0 n (gen_modn1_0 n r hh) hl
+  Definition gen_modn1_0_aux n (modn1:w -> word w n -> w) r h :=
+   let (hh,hl) := gen_split w_0 n h in modn1 (modn1 r hh) hl.
+
+  Fixpoint gen_modn1_0 (n:nat) : w -> word w n -> w :=
+   match n return w -> word w n -> w with
+   | O => fun r x => snd (w_div21 r x b2p)
+   | S n => gen_modn1_0_aux n (gen_modn1_0 n)
    end.
 
   Lemma spec_gen_modn1_0 : forall n r x,
      gen_modn1_0 n r x = snd (gen_divn1_0 n r x).
   Proof.
    induction n;simpl;intros;trivial.
-   destruct (split n x) as (hh,hl).
-   rewrite (IHn r hh).
+   unfold gen_modn1_0_aux, gen_divn1_0_aux.
+   destruct (gen_split w_0 n x) as (hh,hl).
+   rewrite (IHn r hh). 
    destruct (gen_divn1_0 n r hh) as (qh,rh);simpl.
-   rewrite IHn.
-   destruct (gen_divn1_0 n rh hl);trivial.
+   rewrite IHn. destruct (gen_divn1_0 n rh hl);trivial.
   Qed.
  
   Variable p : positive.
   Variable p_bounded : Zpos p < Zpos w_digits.
-  Let add_mul_divp := w_add_mul_div p.
 
   Lemma spec_add_mul_divp : forall x y,
-    [| add_mul_divp x y |] =
+    [| w_add_mul_div p x y |] =
        ([|x|] * (Zpower 2 (Zpos p)) +
           [|y|] / (Zpower 2 ((Zpos w_digits) - (Zpos p)))) mod wB.
   Proof.
-   intros;unfold add_mul_divp;apply spec_add_mul_div;auto.
+   intros;apply spec_add_mul_div;auto.
   Qed.
 
-  Fixpoint gen_divn1_p (n:nat) (r:w) {struct n} : 
-	word w n -> word w n -> word w n * w :=
-   match n return word w n -> word w n ->  word w n * w with
-   | O => fun h l => w_div21 r (add_mul_divp h l) b2p 
-   | S n =>
-     fun (h l:zn2z (word w n)) =>
-      let (hh,hl) := split n h in
-      let (lh,ll) := split n l in	
-      let (qh,rh) := gen_divn1_p n r hh hl in
-      let (ql,rl) := gen_divn1_p n rh hl lh in
-      (genWW n qh ql, rl)
+  Definition gen_divn1_p_aux n 
+   (divn1 : w -> word w n -> word w n -> word w n * w) r h l := 
+   let (hh,hl) := gen_split w_0 n h in
+   let (lh,ll) := gen_split w_0 n l in	
+   let (qh,rh) := divn1 r hh hl in
+   let (ql,rl) := divn1 rh hl lh in
+   (gen_WW w_WW n qh ql, rl).
+
+  Fixpoint gen_divn1_p (n:nat) : w -> word w n -> word w n -> word w n * w :=
+   match n return w -> word w n -> word w n ->  word w n * w with
+   | O => fun r h l => w_div21 r (w_add_mul_div p h l) b2p 
+   | S n => gen_divn1_p_aux n (gen_divn1_p n)   
    end.
 
   Lemma p_lt_gen_digits : forall n, Zpos p < Zpos (gen_digits w_digits n).
   Proof.
-   assert (tmp: 0 < Zpos p); try (red; simpl; auto; fail).
-   induction n;simpl.
-   auto with zarith.
-   change (Zpos (xO (gen_digits w_digits n))) with (2*(Zpos (gen_digits w_digits n)));
-    auto with zarith.
+   induction n;simpl. destruct p_bounded;trivial.
+   assert (0 < Zpos p). unfold Zlt;reflexivity.
+   rewrite Zpos_xO;auto with zarith.
   Qed.
 
   Lemma spec_gen_divn1_p : forall n r h l,
@@ -203,15 +150,14 @@ Section GENDIVN1.
         mod gen_wB w_digits n = [!n|q!] * [|b2p|] + [|r'|] /\
     0 <= [|r'|] < [|b2p|].
   Proof.
-   assert (tmp: 0 < Zpos p); try (red; simpl; auto; fail).
    induction n;intros.
-   unfold gen_divn1_p, gen_to_Z, gen_wB, gen_digits.
+   unfold gen_divn1_p, gen_divn1_p_aux, gen_to_Z, gen_wB, gen_digits.
    rewrite <- spec_add_mul_divp.
-   exact (spec_div21 (add_mul_divp h l) b2p_le H).
-   unfold gen_divn1_p;fold gen_divn1_p.
-   assert (H1 := spec_split n h);destruct (split n h) as (hh,hl).
+   exact (spec_div21 (w_add_mul_div p h l) b2p_le H).
+   unfold gen_divn1_p,gen_divn1_p_aux;fold gen_divn1_p.
+   assert (H1 := spec_split n h);destruct (gen_split w_0 n h) as (hh,hl).
    rewrite H1. rewrite <- gen_wB_wwB.
-   assert (H2 := spec_split n l);destruct (split n l) as (lh,ll).
+   assert (H2 := spec_split n l);destruct (gen_split w_0 n l) as (lh,ll).
    rewrite H2.
    replace ([|r|] * (gen_wB w_digits n * gen_wB w_digits n) +
     (([!n|hh!] * gen_wB w_digits n + [!n|hl!]) * 2 ^ Zpos p +
@@ -237,7 +183,7 @@ Section GENDIVN1.
       gen_wB w_digits n)). 2:ring.
    generalize (IHn rh hl lh H0);destruct (gen_divn1_p n rh hl lh) as (ql,rl);
    intros (H5,H6);rewrite H5.
-   split;[rewrite spec_genWW;ring|trivial]. 
+   split;[rewrite spec_gen_WW;trivial;ring|trivial]. 
    assert (Uhh := spec_gen_to_Z w_digits w_to_Z spec_to_Z n hh);
     unfold gen_wB,base in Uhh.
    assert (Uhl := spec_gen_to_Z w_digits w_to_Z spec_to_Z n hl);
@@ -250,20 +196,13 @@ Section GENDIVN1.
    assert (UU:=p_lt_gen_digits n).
    rewrite Zdiv_shift_r;auto with zarith. 
    2:change (Zpos (gen_digits w_digits (S n))) 
-     with (2*Zpos (gen_digits w_digits n)).
-   2:auto with zarith.
+     with (2*Zpos (gen_digits w_digits n));auto with zarith.
    replace (2 ^ (Zpos (gen_digits w_digits (S n)) - Zpos p)) with
     (2^(Zpos (gen_digits w_digits n) - Zpos p)*2^Zpos (gen_digits w_digits n)).
    rewrite Zdiv_Zmult_compat_r;auto with zarith.
-   replace 
-    ((gen_to_Z w_digits w_to_Z n hh*2^Zpos (gen_digits w_digits n) + 
-         gen_to_Z w_digits w_to_Z n hl) * 2 ^ Zpos p)
-   with 
-    (gen_to_Z w_digits w_to_Z n hh * 2^Zpos(gen_digits w_digits n)*2^Zpos p + 
-      gen_to_Z w_digits w_to_Z n hl*2^Zpos p).
-   2:ring.
-   pattern  (gen_to_Z w_digits w_to_Z n hl * 2 ^ Zpos p) at 2;
-   rewrite (shift_unshift_mod (Zpos (gen_digits w_digits n))(Zpos p)([!n|hl!]));
+   rewrite Zmult_plus_distr_l with (p:=  2^Zpos p). 
+   pattern  ([!n|hl!] * 2^Zpos p) at 2;
+   rewrite (shift_unshift_mod (Zpos(gen_digits w_digits n))(Zpos p)([!n|hl!]));
     auto with zarith.
    rewrite Zplus_assoc. 
    replace 
@@ -287,6 +226,8 @@ Section GENDIVN1.
    rewrite  Zmod_Zmult_compat_l;auto with zarith.
    ring. 
    rewrite Zpower_exp;auto with zarith.
+   assert (0 < Zpos (gen_digits w_digits n)). unfold Zlt;reflexivity.
+   auto with zarith.
    apply Z_mod_lt;auto with zarith.
    rewrite Zpower_exp;auto with zarith.
    split;auto with zarith.
@@ -294,6 +235,7 @@ Section GENDIVN1.
    rewrite <- Zpower_exp;auto with zarith.
    replace (Zpos p + (Zpos (gen_digits w_digits n) - Zpos p)) with 
      (Zpos(gen_digits w_digits n));auto with zarith.
+   assert (0 < Zpos p). unfold Zlt;reflexivity. auto with zarith.
    rewrite <- Zpower_exp;auto with zarith.
    replace (Zpos (gen_digits w_digits (S n)) - Zpos p) with 
        (Zpos (gen_digits w_digits n) - Zpos p + 
@@ -302,21 +244,23 @@ Section GENDIVN1.
     (2*Zpos (gen_digits w_digits n)). ring.
   Qed.
 
-  Fixpoint gen_modn1_p (n:nat) (r:w) {struct n} : word w n -> word w n -> w :=
-   match n return word w n -> word w n -> w with
-   | O => fun h l => snd (w_div21 r (add_mul_divp h l) b2p) 
-   | S n =>
-     fun (h l:zn2z (word w n)) =>
-      let (hh,hl) := split n h in
-      let (lh,ll) := split n l in	
-      gen_modn1_p n (gen_modn1_p n r hh hl) hl lh
+  Definition gen_modn1_p_aux n (modn1 : w -> word w n -> word w n -> w) r h l:=
+   let (hh,hl) := gen_split w_0 n h in
+   let (lh,ll) := gen_split w_0 n l in	
+   modn1 (modn1 r hh hl) hl lh.
+
+  Fixpoint gen_modn1_p (n:nat) : w -> word w n -> word w n -> w :=
+   match n return w -> word w n -> word w n -> w with
+   | O => fun r h l => snd (w_div21 r (w_add_mul_div p h l) b2p) 
+   | S n => gen_modn1_p_aux n (gen_modn1_p n)
    end.
 
   Lemma spec_gen_modn1_p : forall n r h l ,
     gen_modn1_p n r h l = snd (gen_divn1_p n r h l).
   Proof.
    induction n;simpl;intros;trivial.
-   destruct (split n h) as (hh,hl);destruct (split n l) as (lh,ll).
+   unfold gen_modn1_p_aux, gen_divn1_p_aux.
+   destruct(gen_split w_0 n h)as(hh,hl);destruct(gen_split w_0 n l) as (lh,ll).
    rewrite (IHn r hh hl);destruct (gen_divn1_p n r hh hl) as (qh,rh).
    rewrite IHn;simpl;destruct (gen_divn1_p n rh hl lh);trivial.
   Qed.
@@ -377,35 +321,18 @@ Section GENDIVN1.
   (2*Zpos (gen_digits w_digits n)); auto with zarith.
  Qed.
  
- Let _gen_divn1_0 := gen_divn1_0.
- Let _gen_divn1_p := gen_divn1_p.
-
  Definition gen_divn1 (n:nat) (a:word w n) (b:w) := 
   match w_head0 b with
-  | N0 => _gen_divn1_0 b n w_0 a 
+  | N0 => gen_divn1_0 b n w_0 a 
   | Npos p =>
     let b2p := w_add_mul_div p b w_0 in
     let ha := hight n a in
     let k := Pminus w_digits p in
     let lsr_n := w_add_mul_div k w_0 in 
     let r0 := w_add_mul_div p w_0 ha in
-    let (q,r) := _gen_divn1_p b2p p n r0 a (gen0 n) in
+    let (q,r) := gen_divn1_p b2p p n r0 a (gen_0 w_0 n) in
     (q, lsr_n r)
   end.
-
- Theorem wB_div_2:  2 * (wB / 2) = wB.
- Proof.
-  unfold wB,base.
-  assert (2 ^ Zpos w_digits = 
-              2 * (2 ^ (Zpos w_digits - 1))).
-  pattern 2 at 2; rewrite <- Zpower_exp_1.
-  rewrite <- Zpower_exp; auto with zarith.
-  eq_tac; auto with zarith.
-  case w_digits; compute; intros; discriminate.
-  rewrite H.
-  eq_tac; auto with zarith.
-  rewrite Zmult_comm; apply Z_div_mult; auto with zarith.
- Qed.
 
  Lemma spec_gen_divn1 : forall n a b,
     0 < [|b|] ->
@@ -413,7 +340,7 @@ Section GENDIVN1.
     [!n|a!] = [!n|q!] * [|b|] + [|r|] /\
     0 <= [|r|] < [|b|].
   Proof.
-   intros n a b H. unfold gen_divn1, _gen_divn1_p, _gen_divn1_0.
+   intros n a b H. unfold gen_divn1.
    assert (H0 := spec_head0 H).
    destruct (w_head0 b).
    unfold Z_of_N, Zpower in H0.
@@ -423,7 +350,7 @@ Section GENDIVN1.
    rewrite spec_0 in H2;rewrite Zmult_0_l in H2;rewrite Zplus_0_l in H2.
    exact H2.
    unfold Z_of_N in H0.
-   assert (tmp: 0 < Zpos p); try refine (refl_equal _).
+   assert (HHHH : 0 < Zpos p). unfold Zlt;reflexivity.
    assert (Zpos p < Zpos w_digits).
     destruct (Z_lt_le_dec (Zpos p) (Zpos w_digits));trivial.
     assert (2 ^ Zpos p < wB).
@@ -431,8 +358,7 @@ Section GENDIVN1.
      replace (2 ^ Zpos p) with (2^Zpos p * 1);try (ring;fail).
      apply Zmult_le_compat;auto with zarith.
      assert (wB <= 2^Zpos p).
-     unfold wB,base;apply Zpower_le_monotone;auto with zarith.
-     omega.
+     unfold base;apply Zpower_le_monotone;auto with zarith. omega.
    assert ([|w_add_mul_div p b w_0|] = 2 ^ Zpos p * [|b|]).
     assert (H2 := spec_add_mul_div b w_0 H1).
     rewrite spec_0 in H2;rewrite Zdiv_0 in H2;
@@ -462,12 +388,12 @@ Section GENDIVN1.
     pattern 2 at 1;rewrite <- Zpower_exp_1.
     apply Zpower_le_monotone;split;auto with zarith.
    rewrite <- H2 in H0. 
-   assert (H6:= spec_gen_divn1_p H0 H1 n a (gen0 n) H5).
+   assert (H6:= spec_gen_divn1_p H0 H1 n a (gen_0 w_0 n) H5).
    destruct (gen_divn1_p (w_add_mul_div p b w_0) p n
              (w_add_mul_div p w_0 (hight n a)) a
-             (gen0 n)) as (q,r).
+             (gen_0 w_0 n)) as (q,r).
    assert (U:= spec_gen_digits n).
-   rewrite spec_gen0 in H6;rewrite Zdiv_0 in H6.
+   rewrite spec_gen_0 in H6;trivial;rewrite Zdiv_0 in H6.
    rewrite Zplus_0_r in H6.
    rewrite spec_add_mul_div in H6;auto with zarith.
    rewrite spec_0 in H6;rewrite Zmult_0_l in H6;rewrite Zplus_0_l in H6.
@@ -518,19 +444,16 @@ Section GENDIVN1.
    apply Zpower_lt_0;auto with zarith.
  Qed.
 
- Let _gen_modn1_0 := gen_modn1_0.
- Let _gen_modn1_p := gen_modn1_p.
-
  Definition gen_modn1 (n:nat) (a:word w n) (b:w) := 
   match w_head0 b with
-  | N0 => _gen_modn1_0 b n w_0 a 
+  | N0 => gen_modn1_0 b n w_0 a 
   | Npos p =>
     let b2p := w_add_mul_div p b w_0 in
     let ha := hight n a in
     let k := Pminus w_digits p in
     let lsr_n := w_add_mul_div k w_0 in 
     let r0 := w_add_mul_div p w_0 ha in
-    let r := _gen_modn1_p b2p p n r0 a (gen0 n) in
+    let r := gen_modn1_p b2p p n r0 a (gen_0 w_0 n) in
     lsr_n r
   end.
 
@@ -540,9 +463,9 @@ Section GENDIVN1.
   intros n a b;unfold gen_divn1,gen_modn1.
   destruct (w_head0 b).
   apply spec_gen_modn1_0.
-  unfold _gen_modn1_p, _gen_divn1_p;rewrite spec_gen_modn1_p.
+  rewrite spec_gen_modn1_p.
   destruct (gen_divn1_p (w_add_mul_div p b w_0) p n
-            (w_add_mul_div p w_0 (hight n a)) a (gen0 n));simpl;trivial.
+            (w_add_mul_div p w_0 (hight n a)) a (gen_0 w_0 n));simpl;trivial.
  Qed.
 
  Lemma spec_gen_modn1 : forall n a b, 0 < [|b|] ->
@@ -556,6 +479,3 @@ Section GENDIVN1.
  Qed.
 
 End GENDIVN1. 
- 
-
-
