num/W/W2/W2_basic_spec.v
@@ -9,35 +9,83 @@ Open Local Scope w2_scope.
 
 Lemma w2_to_Z_spec : forall x, 0 <= [|x|] < w2_B.
 Proof
-.
-Admitted.
+fun x =>
+ match x as x return 0 <= [|x|] < w2_B with
+ | OO => conj (Zle_refl 0) (refl_equal Lt)
+ | OI => conj (Zle_0_pos 1) (refl_equal Lt)
+ | IO => conj (Zle_0_pos 2) (refl_equal Lt)
+ | II => conj (Zle_0_pos 3) (refl_equal Lt)
+end.
 
 Lemma w2_of_pos_spec : forall p, Zpos p = (Z_of_N (fst (w2_of_pos p)))*w2_B + [|snd (w2_of_pos p)|].
 Proof
-.
-Admitted.
+fun p0 =>
+ eq_ind_r (fun z : Z => Zpos p0 = z + [|snd (w2_of_pos p0)|])
+ match p0 as p0 return Zpos p0 = w2_B*(Z_of_N (fst (w2_of_pos p0))) + [|snd (w2_of_pos p0)|] with
+ | xH => refl_equal (Zpos xH)
+ | xO p1 =>
+    match p1 as p1 return Zpos (xO p1) = w2_B*(Z_of_N (fst (w2_of_pos (xO p1)))) + [|snd (w2_of_pos (xO p1))|] with
+    | xH => refl_equal (Zpos (xO xH))
+    | xO p2 =>
+      refl_equal (Zpos (xO (xO p2)))
+    | xI p2 =>
+      refl_equal (Zpos (xO (xI p2)))
+    end
+ | xI p1 =>
+    match p1 as p1 return Zpos (xI p1) = w2_B*(Z_of_N (fst (w2_of_pos (xI p1)))) + [|snd (w2_of_pos (xI p1))|] with
+    | xH => refl_equal (Zpos (xI xH))
+    | xO p2 =>
+      refl_equal (Zpos (xI (xO p2)))
+    | xI p2 =>
+      refl_equal (Zpos (xI (xI p2)))
+    end
+ end (Zmult_comm (Z_of_N (fst (w2_of_pos p0))) w2_B).
 
 Lemma w2_0_spec : [|OO|] = 0.
 Proof
-.
-Admitted.
+(refl_equal 0).
 
 Lemma w2_1_spec : [|OI|] = 1.
 Proof
-.
-Admitted.
+(refl_equal 1).
 
 Lemma w2_Bm1_spec : [|II|] = w2_B - 1.
 Proof
-.
-Admitted.
+(refl_equal 3).
 
 Lemma w2_WW_spec : forall h l, [||w2_WW h l||] = [|h|] * w2_B + [|l|].
 Proof
-.
-Admitted.
+fun h l =>
+ match h as h return [||w2_WW h l||] = [|h|] * w2_B + [|l|] with
+ | OO => 
+    match l as l return [||w2_WW OO l||] = [|OO|] * w2_B + [|l|] with
+    | OO => refl_equal 0
+    | OI => refl_equal 1
+    | IO => refl_equal 2
+    | II => refl_equal 3
+    end
+ | OI => refl_equal ([||w2_WW OI l||])
+ | IO => refl_equal ([||w2_WW IO l||])
+ | II => refl_equal ([||w2_WW II l||])
+ end.
 
-Lemma w2_CW_spec : forall sign c l, interp_carry sign (w2_B*w2_B) (zn2z_to_Z w2_B w2_to_Z) (w2_CW c l) = (interp_carry sign w2_B w2_to_Z c)*w2_B + [|l|].
-Proof.
-Admitted.
+Lemma w2_W0_spec : forall h, [||w2_W0 h||] = [|h|] * w2_B.
+Proof
+fun h =>
+ match h as h return [||w2_W0 h||] = [|h|] * w2_B with
+ | OO => refl_equal 0
+ | OI => refl_equal ([||w2_W0 OI||])
+ | IO => refl_equal ([||w2_W0 IO||])
+ | II => refl_equal ([||w2_W0 II||])
+ end.
+
+Lemma w2_0W_spec : forall l, [||w2_0W l||] = [|l|].
+Proof
+fun l =>
+ match l as l return [||w2_0W l||] = [|l|] with
+ | OO => refl_equal ([||w2_0W OO||])
+ | OI => refl_equal ([||w2_0W OI||])
+ | IO => refl_equal ([||w2_0W IO||])
+ | II => refl_equal ([||w2_0W II||])
+ end.
 
