num/W/W2/W2_compare_spec.v
@@ -8,6 +8,50 @@ Require Import W2_compare.
 
 Lemma w2_compare_spec : forall x y, match w2_compare x y return Prop with  | Eq => [|x|] = [|y|] | Lt => [|x|] < [|y|] | Gt => [|x|] > [|y|] end.
 Proof
-.
-Admitted.
+fun x y =>
+ let typ x y := match w2_compare x y return Prop with  | Eq => [|x|] = [|y|] | Lt => [|x|] < [|y|] | Gt => [|x|] > [|y|] end in
+ match x as x return typ x y with
+ | OO => 
+    match y as y return typ OO y with
+    | OO => refl_equal 0
+    | _ => refl_equal Lt
+    end
+ | OI => 
+    match y as y return typ OI y with
+    | OO => refl_equal Gt
+    | OI => refl_equal 1
+    | _ => refl_equal Lt
+    end
+ | IO => 
+    match y as y return typ IO y with
+    | OO => refl_equal Gt
+    | OI => refl_equal Gt
+    | IO => refl_equal 2
+    | _ => refl_equal Lt
+    end
+ | II => 
+    match y as y return typ II y with
+    | OO => refl_equal Gt
+    | OI => refl_equal Gt
+    | IO => refl_equal Gt
+    | II => refl_equal 3
+    end
+ end.
+
+Lemma false_true_A : forall A:Prop, false = true -> A.
+ intros A H;  discriminate H.
+Qed.
+
+Lemma w2_eq0_spec : forall x, w2_eq0 x = true -> [|x|] = 0.
+Proof
+fun x =>
+ match x as x return w2_eq0 x = true -> [|x|] = 0 with
+ | OO => fun H => refl_equal 0
+ | OI => fun H => false_true_A (
+[|OI|] = 0) H
+ | IO => fun H => false_true_A (
+[|IO|] = 0) H
+ | II => fun H => false_true_A (
+[|II|] = 0) H
+ end.
 
