num/W/W2/W2_sub_carry_c_spec.v
@@ -7,6 +7,35 @@ Require Import W2_sub.
 
 Lemma w2_sub_carry_c_spec : forall x y, [-|w2_sub_carry_c x y|] = [|x|] - [|y|] - 1.
 Proof
-.
-Admitted.
+fun x y =>
+ match y as y return [-|w2_sub_carry_c x y|] = [|x|] - [|y|] - 1 with
+ | OO =>
+    match x as x return [-|w2_sub_carry_c x OO|] = [|x|] - [|OO|] - 1 with
+    | OO => refl_equal (-1)
+    | OI => refl_equal (0)
+    | IO => refl_equal (1)
+    | II => refl_equal (2)
+   end
+ | OI =>
+    match x as x return [-|w2_sub_carry_c x OI|] = [|x|] - [|OI|] - 1 with
+    | OO => refl_equal (-2)
+    | OI => refl_equal (-1)
+    | IO => refl_equal (0)
+    | II => refl_equal (1)
+   end
+ | IO =>
+    match x as x return [-|w2_sub_carry_c x IO|] = [|x|] - [|IO|] - 1 with
+    | OO => refl_equal (-3)
+    | OI => refl_equal (-2)
+    | IO => refl_equal (-1)
+    | II => refl_equal (0)
+   end
+ | II =>
+    match x as x return [-|w2_sub_carry_c x II|] = [|x|] - [|II|] - 1 with
+    | OO => refl_equal (-4)
+    | OI => refl_equal (-3)
+    | IO => refl_equal (-2)
+    | II => refl_equal (-1)
+   end
+ end.
 
